---
Alias: []
---
> [!Info]
> Subject:: [[Calculus]]
> Parents:: 
> Friends:: 
> Children:: [[Derivative Sum Rule|Sum Rule]] [[Derivative Constant Multiple Rule|Constant Multiple Rule]] [[Derivative Product Rule|Product Rule]] [[Derivative Quotient Rule|Quotient Rule]] [[E|E Rule]] [[Logarithm Derivative Rules]]
---
- ## Basic Rules
  
  - > [!Derivative of a Constant]
  > If $f(x)=k$ where $k$ is **constant**, is [[Derivative|Differentiable]] then:
  > $$\frac{d}{dx}(k)=0$$
  > > [!Proof]-
  > > Step|Explanation
  > > ---|---
  > > $\frac{d}{dx}f(k)=^{lim}_{h\rightarrow 0}\frac{f(x-h)-f(x)}{h}$|Definition of a [[Derivative]]
  > > $\frac{d}{dx}f(k)=^{lim}_{h\rightarrow 0}\frac{k-k}{h}$|No matter what is plugged into $f(k)$ it will always be $k$
  > > $\frac{d}{dx}f(k)=^{lim}_{h\rightarrow 0}\frac{0}{h}$|Simplify
  > > $\frac{d}{dx}f(k)=0$|No matter what $h$ is, $\frac{0}{anything}=0$
  
  - > [!Derivative of x]
  > If $f(x)=x$ is [[Derivative|Differentiable]] then:
  > $$\frac{d}{dx}(x)=1$$
  > > [!Proof]-
  > > Step|Explanation
  > > ---|---
  > > $\frac{d}{dx}f(x)=^{lim}_{h\rightarrow 0}\frac{f(x-h)-f(x)}{h}$|Definition of a [[Derivative]]
  > > $\frac{d}{dx}f(x)=^{lim}_{h\rightarrow 0}\frac{x+h-x}{h}$|Plug the values into $f(x)$
  > > $\frac{d}{dx}f(x)=^{lim}_{h\rightarrow 0}\frac{h}{h}$|Simplify
  > > $\frac{d}{dx}f(x)=1$|Simplify
  
  - ![[Derivative Sum Rule#^4d2afd|Sum Rule]]
  - ![[Derivative Constant Multiple Rule#^59944b|Constant Multiple Rule]]
  - ![[Derivative Product Rule#^e36c72|Product Rule]]
  - ![[Derivative Quotient Rule#^11e7f0|Quotient Rule]]
  - ![[E#^97869e]]
---
- ## Reference